floyd/reptype_lemmas.v
@@ -434,6 +434,12 @@ Inductive pointer_val : Type :=
   | ValidPointer: block -> int -> pointer_val
   | NullPointer.
 
+Lemma PV_eq_dec: forall x y: pointer_val, {x = y} + {x <> y}.
+Proof.
+  intros; destruct x, y; [| right | right | left]; try congruence.
+  destruct (block_eq_dec b b0), (Int.eq_dec i i0); [left | right | right | right]; congruence.
+Qed.
+
 Definition pointer_val_val (pv: pointer_val): val :=
   match pv with
   | ValidPointer b i => Vptr b i
